approach.thy
@@ -1,5 +1,6 @@
 theory approach
 imports Main sem1_commutativity
+  replissSem_singleSession
 begin
 
 
@@ -13,6 +14,44 @@ TODO:
 3. other things
 
 *)
+
+
+
+text {*
+When a program is correct in the single session semantics, 
+it is also correct when executed in the concurrent interleaving semantics.
+*}
+theorem
+assumes works_in_single_session: "programCorrect_s program"
+shows "programCorrect program"
+proof (rule show_programCorrect_noTransactionInterleaving)
+  text {* Assume we have a trace and a final state S *}
+  fix trace S
+  text {* Such that executing the trace finishes in state S. *}
+  assume steps: "initialState program ~~ trace \<leadsto>* S"
+  
+  text {* We can assume transactions are packed. *}
+  assume packed: "transactionsArePacked trace"
+  
+  text {* We show that the trace must be correct (proof by contradiction). *}
+  show "traceCorrect program trace"
+  proof (rule ccontr)
+    assume incorrect_trace: "\<not> traceCorrect program trace"
+    
+    text {* If the trace is incorrect, there must be a failing invariant check in the trace: *}
+    from this obtain s where "(s, AInvcheck False) \<in> set trace"
+       using steps by (auto simp add: traceCorrect_def)
+    
+       
+   (* TODO now we need to split up the transactions one by one *)    
+    
+    
+  
+  
+
+
+qed
+
 
 
 end
